Root2/Prime/PrimeFactor.lean
@@ -21,13 +21,211 @@ def List.anyP (list: List a) (P : a -> Prop) : Prop := match list with
   | x :: xs => P x ∨ anyP xs P
 
 @[simp]
-def List.sorted (list: List a) (P : a -> a -> Prop) : Prop := match list with
+def List.sorted_by (list: List a) (P : a -> a -> Prop) : Prop := match list with
   | [] | [_] => True
-  | a :: b :: xs => P a b ∧ sorted (b :: xs) P
+  | a :: b :: xs => P a b ∧ sorted_by (b :: xs) P
+
+@[simp]
+def List.sorted (list: List nat) : Prop := match list with
+  | [] | [_] => True
+  | a :: b :: xs => b <= a ∧ sorted (b :: xs)
+
+@[simp]
+def List.concat_sorted (a b: List nat) : List nat := match a with
+| [] => b
+| a₀::as => match b with
+| [] => a₀::as
+| b₀::bs => if a₀ <= b₀ then b₀::(List.concat_sorted (a₀::as) bs) else a₀::(List.concat_sorted as (b₀::bs))
+termination_by List.concat_sorted a b => (a, b)
+
+theorem pop_sorted {{a: nat}} {{as: List nat}} : (a::as).sorted -> as.sorted := by
+  intro list_sorted
+  match as with
+  | [] => trivial
+  | a₀::as₀ => exact list_sorted.right
+
+theorem singleton_list_is_sorted {a: nat} : [a].sorted := by simp
+
+theorem list_concat_sorted_fst (b_lt_a: b < a) : List.concat_sorted (a::as) (b::bs) = a :: (List.concat_sorted as (b::bs)) := by
+  simp
+  split
+  have := nat.comp_dec b_lt_a (by assumption)
+  contradiction
+  rfl
+
+theorem list_concat_sorted_snd (_: a <= b) : List.concat_sorted (a::as) (b::bs) = b :: (List.concat_sorted (a::as) bs) := by
+  simp
+  split
+  rfl
+  contradiction
+
+theorem concat_sorted_is_correct (a b: List nat) (a_sorted: a.sorted) (b_sorted: b.sorted) : 
+  (a.concat_sorted b).sorted := by
+  unfold List.concat_sorted
+  match a, b with
+  | [], _ =>
+    simp
+    assumption
+  | _, [] =>
+    simp
+    split
+    simp
+    assumption
+  | [a₀], [b₀] =>
+    simp
+    split
+    {
+      simp
+      assumption
+    }
+    {
+      simp
+      have b₀_lt_a₀ : b₀ < a₀ := by
+        rw [←nat.not_le_is_sym_lt]
+        assumption
+      exact (nat.lt_is_le _ _ b₀_lt_a₀)
+    }
+  | [a₀], b₀::b₁::bs =>
+    simp
+    split <;> simp
+    split <;> simp
+    apply And.intro
+    exact b_sorted.left
+    rw [←list_concat_sorted_snd]
+    apply concat_sorted_is_correct
+    repeat assumption
+    exact b_sorted.right
+    assumption
+    apply And.intro
+    assumption
+    apply And.intro
+    apply nat.not_le_implies_le_symm
+    assumption
+    exact b_sorted.right
+    apply And.intro
+    apply nat.not_le_implies_le_symm
+    assumption
+    apply And.intro
+    exact b_sorted.left
+    exact b_sorted.right
+  | a₀::a₁::as, [b₀] =>
+    simp
+    split <;> simp
+    apply And.intro <;> assumption
+    split <;> simp
+    repeat any_goals apply And.intro
+    repeat any_goals (apply nat.not_le_implies_le_symm; assumption)
+    repeat any_goals assumption
+    any_goals exact a_sorted.left
+    any_goals exact a_sorted.right
+    rw [←list_concat_sorted_fst]
+    apply concat_sorted_is_correct
+    repeat any_goals apply And.intro
+    repeat any_goals (apply nat.not_le_implies_le_symm; assumption)
+    repeat any_goals (rw [←nat.not_le_is_sym_lt]; assumption)
+    repeat any_goals assumption
+    any_goals exact a_sorted.right
+  | a₀::a₁::as, b₀::b₁::bs =>
+    unfold List.concat_sorted
+    simp
+    split <;> simp <;> split <;> simp
+    {
+      apply And.intro
+      repeat assumption
+      exact b_sorted.left
+      rw [←list_concat_sorted_snd]
+      apply concat_sorted_is_correct
+      repeat assumption
+      exact b_sorted.right
+      repeat assumption
+    }
+    {
+      apply And.intro
+      assumption
+      split <;> simp
+      {
+        apply And.intro
+        apply nat.not_le_implies_le_symm
+        assumption
+        rw [←list_concat_sorted_snd]
+        apply concat_sorted_is_correct
+        exact a_sorted.right
+        exact b_sorted.right
+        repeat assumption
+      }
+      {
+        apply And.intro
+        exact a_sorted.left
+        rw [←list_concat_sorted_fst]
+        apply concat_sorted_is_correct
+        exact a_sorted.right
+        exact b_sorted.right
+        rw [←nat.not_le_is_sym_lt]
+        assumption
+      }
+    }
+    {
+      apply And.intro
+      apply nat.not_le_implies_le_symm
+      assumption
+      split
+      simp
+      apply And.intro
+      exact b_sorted.left
+      rw [←list_concat_sorted_snd]
+      apply concat_sorted_is_correct
+      exact a_sorted.right
+      exact b_sorted.right
+      assumption
+      simp
+      apply And.intro
+      assumption
+      rw [←list_concat_sorted_fst]
+      apply concat_sorted_is_correct
+      exact a_sorted.right
+      exact b_sorted.right
+      rw [←nat.not_le_is_sym_lt]
+      assumption
+    }
+    {
+      apply And.intro
+      exact a_sorted.left
+      rw [←list_concat_sorted_fst]
+      apply concat_sorted_is_correct
+      exact a_sorted.right
+      assumption
+      rw [←nat.not_le_is_sym_lt]
+      assumption
+    }
+  termination_by concat_sorted_is_correct => a.length + b.length
+  decreasing_by {
+    simp_wf
+    try { exact Nat.add_lt_add_left (Nat.lt_succ_self _) (Nat.succ 0) }
+    try { exact Nat.add_lt_add_right (Nat.lt_succ_self _) (Nat.succ 0) }
+    try {
+      repeat rw [Nat.succ_add]
+      rw [Nat.add_comm _ (Nat.succ _)]
+      repeat rw [Nat.succ_add]
+      rw [Nat.add_comm _ (Nat.succ _)]
+      repeat rw [Nat.succ_add]
+      repeat apply Nat.succ_lt_succ
+      repeat rw [←Nat.succ_add]
+      apply Nat.add_lt_add_right
+      apply Nat.le_succ
+    }
+    try {
+      repeat rw [Nat.succ_add]
+      rw [Nat.add_comm _ (Nat.succ _)]
+      rw [Nat.succ_add]
+      apply Nat.succ_lt_succ
+      apply Nat.lt_succ_self
+    }
+  }
 
 inductive PrimeFactorization (n: nat) : Type :=
   | PrimeFactors : (factors: List nat)
     -> List.allP factors nat.prime
+    -> factors.sorted
     -> n = list_product factors
     -> PrimeFactorization n 
 
@@ -109,7 +307,7 @@ def prime_gt_zero (n: nat) (_: nat.prime n) : nat.zero < n := match n with
   | nat.inc _ => nat.zero_lt_inc _
 
 def PrimeFactorization.to_list (p: PrimeFactorization n) : List nat := match p with
-  | .PrimeFactors factors _ _ => factors
+  | .PrimeFactors factors _ _ _ => factors
 
 instance : Repr (PrimeFactorization n) where
   reprPrec n := reprPrec n.to_list
@@ -119,9 +317,13 @@ def PrimeFactorization.merge {{a b: nat}}
   (pb: PrimeFactorization b) :
   PrimeFactorization (nat.mul a b) := by
   match pa, pb with
-  | .PrimeFactors a_products a_primes a_product, .PrimeFactors b_products b_primes b_product =>
+  | .PrimeFactors a_products a_primes a_sorted a_product, .PrimeFactors b_products b_primes b_sorted b_product =>
     apply PrimeFactorization.PrimeFactors (a_products ++ b_products)
     apply concat_preserves_all <;> assumption
+    {
+
+      admit
+    }
     {
       rw [a_product, b_product]
       apply mul_list_products
@@ -141,6 +343,7 @@ def nat.factorize (n: nat) (_: nat.zero < n) : PrimeFactorization n := by
       apply PrimeFactorization.PrimeFactors [n]
       simp
       assumption
+      simp
       simp
       rw [nat.mul_one_r]
     | .Composite _ composite =>
